promise_free/examples/MPIA.v
@@ -7,122 +7,105 @@ Module MPIA. Section MPIA.
   Context `{!crisG Γ Σ α β τ _S _I, !concG, !histG, !atomicG, !sysG, !one_shotG}.
   Local Existing Instances one_shot_inG.
 
-  Definition Ist : alist key Any.t → alist key Any.t → iProp Σ := λ _ _, emp%I.
+  Definition Ist : ist_type Σ := λ _ _, emp%I.
 
-  Context (sp_user : spl_type).
-  Context (sp_s : sp_type).
-  Context (SchInSpS : sp_incl (SystemA.sp sp_user ⊤) sp_s).
-  Context (HMP : spl_sub MPA.sp sp_user).
+  Context (sp_s sp_user : specmap).
+  Context (SchInSpS : (SystemA.sp sp_user ⊤) ⊆ sp_s).
+  Context (HMP : MPA.sp ⊆ sp_user).
 
-  Local Definition MA := (MPA.t sp_s ★ SystemA.t sp_user sp_s ★ PFMemA.t sp_s).
-  Local Definition MI := (MPI.t      ★ SystemA.t sp_user sp_s ★ PFMemA.t sp_s).
+  Local Definition MA := (MPA.t sp_s ★ SystemA.t sp_user ⊤ sp_s ★ PFMemA.t sp_s).
+  Local Definition MI := (MPI.t      ★ SystemA.t sp_user ⊤ sp_s ★ PFMemA.t sp_s).
   Local Definition IstFull := (IstProd (IstSB (Mod.scopes (MPA.t sp_s)) Ist) IstEq).
 
-  Lemma mp2_spawnable : SystemA.fspec_spawnable sp_user MPHdr.mp2 MPA.mp2_precondition.
+  Lemma mp2_spawnable : ⊢ SystemA.fspec_spawnable sp_user MPHdr.mp2 MPA.mp2_precondition.
   Proof.
-    exists MPA.mp2_spec; split; [eapply HMP; ss|].
-    intros [tid stid]; ss; exists ((tid, stid)); split.
-    { unfold_pre_post. iIntros (??) "[$ [% [-> [% [$ [% [-> P]]]]]]]"; iModIntro; iFrame; ss. }
-    { unfold_pre_post; iIntros (??) "[$ $] //". }
+    iExists MPA.mp2_spec; iSplit; [iPureIntro; eapply lookup_weaken; eauto; by simpl_map|].
+    iIntros "%P %Q [%x [-> ->]]"; iExists _, _; iSplit; [iPureIntro; exists x; split; ss|].
+    unfold_pre_post. destruct x.
+    iIntros (varg arg) "[$ [% [-> [% [$ [% [% $]]]]]]] /= !>"; iSplitL; eauto.
   Qed.
 
-  Lemma simF_mp : ISim.sim_fun open MA MI MPA.init_cond%I IstFull None.
-  Proof.
-    init_simF.
-    (* iDestruct "IST" as "[[-> ->] TV]". *)
-    steps_l. iDestruct "ASM" as "->". hss_l. steps_l.
-    steps_r. hss_r. steps_r.
+  Lemma simF_mp : ISim.sim_fun open MA MI IstFull None.
+  Proof using SchInSpS HMP.
+    iStartSim.
+    steps_l. iDestruct "ASM" as "[-> TV]". rewrite /MPA.mp /MPI.mp; steps_l; steps_r.
 
-    iApply wsim_system_yield; ss.
-    { unfold_sp_exact sp_s SystemHdr.yield; ss. }
-    iFrame "TID". iSplit.
-    { iExists [], [], _, _; iSplit; eauto.
-      iSplit; eauto.
-      iSplit; eauto.
-      iPureIntro; split; unfold_mod; prove_scope.
-    }
-    iFrame.
+    iApply wsim_system_yield_ir; ss.
+    { simpl_sp; auto. }
+    iFrame "TV IST".
     iIntros (??) "IST TV".
-    Unshelve. all: try exact ⊤.
 
     (* alloc *)
     steps_r. inline_r. force_r (1%positive, 0, 2, _). forces_r. iFrame. iSplit; eauto.
-    steps_r. iDestruct "GRT" as "[[%loc [%V' [[-> %LE] [TV [FA ↦]]]]] ->]".
+    steps_r. iDestruct "GRT" as "[-> [%loc [%V' [[-> %LE] [TV [FA ↦]]]]]]".
     rewrite own_loc_na_vec_cons own_loc_na_vec_singleton.
     hss_r. steps_r.
 
     (* yield *)
-    iApply wsim_system_yield; ss.
-    { unfold_sp_exact sp_s SystemHdr.yield; ss. }
+    iApply wsim_system_yield_ir; ss.
+    { simpl_sp; auto. }
     iFrame "TV IST".
     clear dependent st_src st_tgt.
-    iIntros (??) "IST TV".
-    Unshelve. all: try exact ⊤.
+    iIntros (??) "IST TV". steps_r.
 
     (* yield *)
-    steps_r.
-    iApply wsim_system_yield; ss.
-    { unfold_sp_exact sp_s SystemHdr.yield; ss. }
+    iApply wsim_system_yield_ir; ss.
+    { simpl_sp; auto. }
     iFrame "TV IST".
     clear dependent st_src st_tgt.
-    iIntros (??) "IST TV".
-    Unshelve. all: try exact ⊤.
+    iIntros (??) "IST TV". steps_r.
 
     (* write *)
-    steps_r. inline_r.
-    force_r (existT 0 (1%positive, 0, loc, Val.Vnum 0, Ordering.na, _)). forces_r.
-    rewrite shift_0.
+    inline_r.
+    unshelve force_r (FSpec_mk _ _ (or_introl _)); last steps_r.
+    3:{ eexists (1%positive, 0, loc, Val.Vnum 0, Ordering.na, _). split; ss. }
+    rewrite shift_0. forces_r.
     iFrame "TV".
     iDestruct "↦" as "[↦flag ↦data]"; iSplitL "↦flag".
     { do 2 (iSplit; eauto). iApply own_loc_na_own_loc; done. }
-    steps_r. iDestruct "GRT" as "[[%V'' [[-> %HLE2] [↦flag TV]]] ->]". hss_r.
+    steps_r. iDestruct "GRT" as "[-> [%V'' [[-> %HLE2] [↦flag TV]]]]". hss_r.
     tview_sync HLE2.
     steps_r.
 
     (* yield *)
-    steps_r.
-    iApply wsim_system_yield; ss.
-    { unfold_sp_exact sp_s SystemHdr.yield; ss. }
+    iApply wsim_system_yield_ir; ss.
+    { simpl_sp; auto. }
     iFrame "TV IST".
     clear dependent st_src st_tgt.
     iIntros (??) "IST TV".
-    Unshelve. all: try exact ⊤.
 
     (* write *)
     steps_r. inline_r.
-    force_r (existT 0 (1%positive, 0, loc >> 1, Val.Vnum 0, Ordering.na, _)). forces_r.
+    unshelve force_r (FSpec_mk _ _ (or_introl _)); last forces_r.
+    3:{ eexists (1%positive, 0, loc >> 1, Val.Vnum 0, Ordering.na, _). split; ss. }
     iPoseProof (own_loc_na_own_loc with "↦data") as "$".
     iFrame "TV".
     iSplit; eauto.
-    steps_r. iDestruct "GRT" as "[[%V3 [[-> %Hle3] [↦data TV]]] ->]".
+    steps_r. iDestruct "GRT" as "[-> [%V3 [[-> %Hle3] [↦data TV]]]]".
     tview_sync Hle3. hss_r. steps_r.
 
     (* yield *)
-    steps_r.
-    iApply wsim_system_yield; ss.
-    { unfold_sp_exact sp_s SystemHdr.yield; ss. }
+    iApply wsim_system_yield_ir; ss.
+    { simpl_sp; auto. }
     iFrame "TV IST".
     clear dependent st_src st_tgt.
     iIntros (??) "IST TV".
-    Unshelve. all: try exact ⊤.
 
     (* spawn *)
     iMod (own_alloc Pending) as "[%γ O]"; ss.
     iMod (AtomicPtsTo_from_na loc (Val.Vnum 0) with "↦flag")
       as "[%γx [% [% [% [% [% [% [SW ↦flag]]]]]]]]".
     iMod (inv_alloc (MPA.mp_inv' 0 loc (loc >> 1) γ γx) 1 _ _ MPA.mpN with "[↦flag]") as "#I"; eauto.
-    { rewrite MPA.mp_inv'_eq.
-      SL_red; iExists _; SL_red; iExists false.
-      do 6 (SL_red; iExists _).
-      SL_red; iSplit; last done.
-      rewrite syn_AtomicPtsTo_red; iFrame.
+    { rewrite MPA.mp_inv'_eq. solve_base_sl_red. iExists _, false, _, _, _, _, _, _.
+      solve_base_sl_red; iFrame.
+      iSplitL; first rewrite syn_AtomicPtsTo_red; iFrame.
+      solve_base_sl_red.
     }
     iPoseProof (AtomicSWriter_AtomicSeen with "SW") as "#SN".
 
     (* source yield *)
     iApply wsim_system_yield_src.
-    force_l (Val.Vptr loc). steps_l.
-    (* iApply wsim_system_yield_src. steps_l. *)
+    force_l (Val.Vptr loc). steps_l. simpl_sp.
 
     (* spawn *)
     force_l (1%positive, 0, MPA.mp2_precondition, V3). forces_l.
@@ -131,19 +114,18 @@ Module MPIA. Section MPIA.
     { iExists _; iSplit; first done.
       iExists _, _, _; iSplit; first (iPureIntro; esplits; eauto using mp2_spawnable).
       rewrite /MPA.mp2_precondition /MPA.mp_inv; iFrame "↦data SW".
-      iExists γ; iSplit; eauto.
-      rewrite shift_0; eauto.
+      iSplitR; first iApply mp2_spawnable.
+      iExists γ; iSplit; eauto. rewrite shift_0; eauto.
     }
     steps_l. steps_r. call "IST".
 
+    clear dependent st_src st_tgt. iIntros (ret st_src st_tgt) "IST".
     steps_l. iDestruct "ASM" as "[% [-> [TV [-> ->]]]]".
-    steps_r. hss_r. steps_r.
-    clear dependent st_src st_tgt.
+    steps_r. hss_r. steps_r. hss_l; steps_l.
     iApply wsim_reset.
-    (* iRevert "I FA O SW IST TV". *)
     iStopProof.
 
-    revert st_s'. combine_quant st_t'. clear Hle3 H4. combine_quant V3.
+    revert st_src. combine_quant st_tgt. clear Hle3 H6. combine_quant V3.
     eapply wsim_coind.
     (* destruct_quant. *)
     iIntros (g' _ CIH [V3 [st_t st_s]]) "[#[I SN] [FA [P [IST TV]]]]"; s.
@@ -153,51 +135,46 @@ Module MPIA. Section MPIA.
 
     (* yield *)
     steps_r.
-    iApply wsim_system_yield; ss.
-    { unfold_sp_exact sp_s SystemHdr.yield; ss. }
+    iApply wsim_system_yield_ir; ss. { simpl_sp; auto. }
     iFrame "TV IST".
     clear dependent st_s st_t.
     iIntros (??) "IST TV".
-    Unshelve. all: try exact ⊤.
 
     steps_r. inline_r.
     iInv "I" as "INV" "ACC".
-    iEval (rewrite MPA.mp_inv'_eq /MPA.mp_inv'_def; SL_red) in "INV".
-    do 8 (iDestruct "INV" as "[% INV]"; iEval (SL_red) in "INV").
+    iEval (rewrite MPA.mp_inv'_eq /MPA.mp_inv'_def; solve_base_sl_red) in "INV".
+    iDestruct "INV" as "[% [%x0 [% [% [% [% [% [% [↦flag H]]]]]]]]]".
     destruct x0; cycle 1.
     { (* read 0 from flag *)
-      iEval (SL_red; rewrite syn_AtomicPtsTo_red) in "INV"; iDestruct "INV" as "[↦flag ->]".
-      rewrite AtomicPtsTo_eq. iDestruct "↦flag" as "[% ↦flag]".
-      force_r (existT 1 (1%positive, 0, loc, Ordering.acqrel, _, _, _, _, _, _, _, _)). forces_r.
-      iFrame "TV SN ↦flag". iSplit; eauto.
+      iEval (rewrite syn_AtomicPtsTo_red AtomicPtsTo_eq /AtomicPtsTo_def) in "↦flag".
+      iDestruct "↦flag" as "[% ↦flag]".
+      iEval (solve_base_sl_red) in "H"; iPoseProof "H" as "->".
+      unshelve force_r (FSpec_mk _ _ (or_intror _)); last steps_r.
+      3:{ eexists (1%positive, 0, loc, Ordering.acqrel, _, _, _, γx, _, _, _, z1). split; ss. }
+      forces_r.
+      iFrame "TV SN ↦flag". iSplit; auto.
       steps_r.
-      iDestruct "GRT" as "[[% [% [% [% [% [% [%V4 [[-> %] [#SN2 [↦flag TV]]]]]]]]]] ->]".
+      iDestruct "GRT" as "[-> [% [% [% [% [% [% [%V4 [[-> %] [#SN2 [↦flag TV]]]]]]]]]]]".
       hss_r. steps_r.
       iMod ("ACC" with "[↦flag]") as "_".
-      { rewrite {2}MPA.mp_inv'_eq; SL_red; iExists _.
-        SL_red; iExists false.
-        do 6 (SL_red; iExists _); SL_red.
+      { rewrite {2}MPA.mp_inv'_eq; solve_base_sl_red; iExists _, false. repeat iExists _.
         rewrite syn_AtomicPtsTo_red AtomicPtsTo_eq /AtomicPtsTo_def; iFrame.
-        done.
+        solve_base_sl_red.
       }
 
-      steps_r.
-      iApply wsim_system_yield; ss.
-      { unfold_sp_exact sp_s SystemHdr.yield; ss. }
+      iApply wsim_system_yield_ir; ss. { simpl_sp; auto. }
       iFrame "TV IST".
       clear dependent st_src st_tgt.
       iIntros (??) "IST TV".
 
-      steps_r.
-      hexploit (H6 (Cell.max_ts ζ'')); first done; rewrite Cell.singleton_get.
+      steps_r. des.
+      hexploit (H8 (Cell.max_ts ζ'')); first done; rewrite Cell.singleton_get.
       des_if; intros INV; inv INV.
       destruct v'; ss.
-      apply Z.eqb_eq in H4; subst.
+      apply Z.eqb_eq in H6; subst.
       steps_r.
 
-      steps_r.
-      iApply wsim_system_yield; ss.
-      { unfold_sp_exact sp_s SystemHdr.yield; ss. }
+      iApply wsim_system_yield_ir; ss. { simpl_sp; auto. }
       iFrame "TV IST".
       clear dependent st_src st_tgt.
       iIntros (??) "IST TV".
@@ -207,24 +184,23 @@ Module MPIA. Section MPIA.
       iApply wsim_progress.
       iApply wsim_base.
       iIntros "W".
-
       iApply ((CIH (V4, (st_tgt, st_src))) with "[-]"); iFrame. iFrame "I".
-      ss. iModIntro. iEval (rewrite H8) in "SN". done.
+      ss. iModIntro. iEval (rewrite H10) in "SN". done.
       Unshelve. all: try exact ⊤; try exact 1%Qp.
     }
     { (* read 1 from flag *)
-      iDestruct "INV" as "[↦flag INV]".
-      do 3 (SL_red; iDestruct "INV" as "[% INV]").
-      SL_red; iDestruct "INV" as "[[% %Hadd] [P2|INV]]".
+      iEval (solve_base_sl_red) in "H".
+      iDestruct "H" as "[% [% [% [[% %Hadd] [P2|INV]]]]]".
       { iCombine "P" "P2" gives %WF; inv WF. }
       rewrite syn_AtomicPtsTo_red.
       iEval (rewrite AtomicPtsTo_eq /AtomicPtsTo_def /view_at) in "↦flag".
       iDestruct "↦flag" as "[% ↦flag]".
-      force_r (existT 1 (_, _, _, _, _, _, _, _, _, _, V3, x2)). forces_r.
+      unshelve force_r (FSpec_mk _ _ (or_intror _)); last steps_r.
+      3:{ eexists (1%positive, 0, loc, Ordering.acqrel, _, _, _, γx, _, _, V3, z1). split; ss. }
       (* iPoseProof (AtomicSWriter_AtomicSeen with "SW") as "#SN". *)
-      iFrame "TV SN ↦flag". iSplit; eauto.
+      forces_r. iFrame "TV SN ↦flag". iSplit; eauto.
       steps_r.
-      iDestruct "GRT" as "[[% [% [% [% [% [% [% [[-> %Hres] [#SN2 [↦flag TV]]]]]]]]]] ->]".
+      iDestruct "GRT" as "[-> [% [% [% [% [% [% [% [[-> %Hres] [#SN2 [↦flag TV]]]]]]]]]]]".
       destruct Hres as [Hval [Hcell1 [Hcell2 [Hget [Hvle Hvle2]]]]].
       hexploit (Hcell2 (Cell.max_ts ζ'')); eauto.
       erewrite Cell.add_o; eauto; des_if.
@@ -234,55 +210,49 @@ Module MPIA. Section MPIA.
         destruct v'; ss. apply Z.eqb_eq in Hval; subst.
         hss_r; steps_r.
         iMod ("ACC" with "[↦flag P]") as "_".
-        { rewrite MPA.mp_inv'_eq; SL_red; iExists _.
-          SL_red; iExists true.
-          do 6 (SL_red; iExists _); SL_red.
+        { rewrite MPA.mp_inv'_eq; solve_base_sl_red.
+          iExists _, true; repeat iExists _.
           rewrite syn_AtomicPtsTo_red AtomicPtsTo_eq /AtomicPtsTo_def; iFrame.
-          do 3 (iExists _; SL_red); iFrame "P"; eauto.
+          solve_base_sl_red; iFrame "P"; auto.
         }
 
         (* yield *)
-        iApply wsim_system_yield; ss.
-        { unfold_sp_exact sp_s SystemHdr.yield; ss. }
+        iApply wsim_system_yield_ir; ss. { simpl_sp; auto. }
         iFrame "TV IST".
         clear dependent st_src st_tgt.
         iIntros (??) "IST TV".
         steps_r.
 
         (* yield *)
-        iApply wsim_system_yield; ss.
-        { unfold_sp_exact sp_s SystemHdr.yield; ss. }
+        iApply wsim_system_yield_ir; ss. { simpl_sp; auto. }
         iFrame "TV IST".
         clear dependent st_src st_tgt.
         iIntros (??) "IST TV".
         steps_r.
-        Unshelve. all: try exact ⊤.
 
         (* yield *)
-        iApply wsim_system_yield; ss.
-        { unfold_sp_exact sp_s SystemHdr.yield; ss. }
+        iApply wsim_system_yield_ir; ss. { simpl_sp; auto. }
         iFrame "TV IST".
         clear dependent st_src st_tgt.
         iIntros (??) "IST TV".
         steps_r.
 
         (* non-atomic load here *)
-        inline_r. force_r (existT 0 (_, _, _, _, _, _, _)). forces_r.
+        inline_r. unshelve force_r (FSpec_mk _ _ (or_introl _)); last steps_r.
+        3:{ eexists (_, _, _, _, _, _, _). split; ss. }
         iEval (rewrite syn_own_loc_na_red) in "INV".
-        assert (Hawk : Ordering.le Ordering.acqrel Ordering.acqrel) by refl.
+        assert (Hawk : Ordering.le Ordering.acqrel Ordering.acqrel) by refl. forces_r.
         rewrite Hvle2 Hawk Hvle.
         iFrame "TV INV". iSplit; eauto.
 
-        steps_r. iDestruct "GRT" as "[[% [% [[-> %Hval'] [↦data TV]]]] ->]". hss_r.
+        steps_r. iDestruct "GRT" as "[-> [% [% [[-> %Hval'] [↦data TV]]]]]". hss_r.
 
         steps_r.
-        iApply wsim_system_yield; ss.
-        { unfold_sp_exact sp_s SystemHdr.yield; ss. }
+        iApply wsim_system_yield_ir; ss. { simpl_sp; auto. }
         iFrame "TV IST".
         clear dependent st_src st_tgt.
         iIntros (??) "IST TV".
         steps_r.
-        Unshelve. all: try exact ⊤.
 
         destruct v'; ss. eapply Z.eqb_eq in Hval'; subst.
         steps_r.
@@ -291,7 +261,6 @@ Module MPIA. Section MPIA.
         forces_l. iSplit; eauto.
         step.
         iSplit; eauto.
-        Unshelve. all: try exact ⊤; try exact 1%Qp.
       }
       { (* read 0 *)
         rewrite Cell.singleton_get; des_if; intros INV; inv INV.
@@ -300,24 +269,21 @@ Module MPIA. Section MPIA.
 
         (* close invariant *)
         iMod ("ACC" with "[↦flag INV]") as "_".
-        { rewrite MPA.mp_inv'_eq; SL_red; iExists _.
-          SL_red; iExists true.
-          do 6 (SL_red; iExists _); SL_red.
+        { iClear "I". rewrite MPA.mp_inv'_eq. iEval solve_base_sl_red. iExists _, true.
+          do 6 iExists _.
           rewrite syn_AtomicPtsTo_red AtomicPtsTo_eq /AtomicPtsTo_def; iFrame.
-          do 3 (iExists _; SL_red); iFrame "INV"; eauto.
+          iEval solve_base_sl_red. iFrame "INV"; eauto.
         }
 
         (* yield *)
-        iApply wsim_system_yield; ss.
-        { unfold_sp_exact sp_s SystemHdr.yield; ss. }
+        iApply wsim_system_yield_ir; ss. { simpl_sp; auto. }
         iFrame "TV IST".
         clear dependent st_src st_tgt.
         iIntros (??) "IST TV".
         steps_r.
 
         (* yield *)
-        iApply wsim_system_yield; ss.
-        { unfold_sp_exact sp_s SystemHdr.yield; ss. }
+        iApply wsim_system_yield_ir; ss. { simpl_sp; auto. }
         iFrame "TV IST".
         clear dependent st_src st_tgt.
         iIntros (??) "IST TV".
@@ -327,78 +293,71 @@ Module MPIA. Section MPIA.
         iApply wsim_progress.
         iApply wsim_base.
         iIntros "W".
-        (* iSpecialize ("CIH" $! ); s. *)
 
         iApply ((CIH (_, (st_tgt, st_src))) with "[-]"); iFrame. iFrame "I".
         iEval (rewrite Hvle) in "SN"; s; iModIntro; done.
       }
     }
   Unshelve. all: try exact 1%Qp; try exact ⊤.
-  (*SLOW*)Admitted.
+  (*SLOW*)Qed.
 
-  Lemma simF_mp2 : ISim.sim_fun open MA MI MPA.init_cond%I IstFull (Some MPHdr.mp2).
-  Proof.
-    init_simF.
-    steps_l.
-    iDestruct "ASM" as "[%va [-> [%sa [%V [-> [PRE TV]]]]]]".
-    rename _q1 into tid, _q2 into stid. hss_l.
-    rewrite /MPA.mp2_precondition.
+  Lemma simF_mp2 : ISim.sim_fun open MA MI IstFull (Some MPHdr.mp2).
+  Proof using SchInSpS HMP.
+    iStartSim.
+    steps_l. destruct _q as [tid stid].
+    iDestruct "ASM" as "[%va [-> [%sa [%V [-> [PRE TV]]]]]]". hss_l.
     iDestruct "PRE" as "[%loc [%γ [%γx [%V0 [%fd [%td [% [% [[-> ->] [#I [↦data ⊒]]]]]]]]]]]".
     steps_l. hss_l. steps_l.
 
     rewrite /MPA.mp2. steps_l.
-
     steps_r. hss_r. steps_r. hss_r. steps_r.
     rewrite /MPI.mp2. norm_r.
 
     (* yield *)
-    iApply wsim_system_yield; ss.
-    { unfold_sp_exact sp_s SystemHdr.yield; ss. }
+    iApply wsim_system_yield_ir; ss. { simpl_sp; ss. }
     iFrame "TV IST".
     clear dependent st_src st_tgt.
     iIntros (??) "IST TV".
     steps_r.
-    Unshelve. all: try exact ⊤.
 
     (* yield *)
-    iApply wsim_system_yield; ss.
-    { unfold_sp_exact sp_s SystemHdr.yield; ss. }
+    iApply wsim_system_yield_ir; ss. { simpl_sp; ss. }
     iFrame "TV IST".
     clear dependent st_src st_tgt.
     iIntros (??) "IST TV".
     steps_r.
-    Unshelve. all: try exact ⊤.
 
     (* write to data *)
-    inline_r.
-    force_r (existT 0 (_, _, _, _, _, _)). forces_r.
+    inline_r. unshelve force_r.
+    { econs; left; eexists (_, _, _, _, _, _). split; ss. }
+    forces_r.
     iPoseProof (own_loc_na_own_loc with "↦data") as "↦data".
     iFrame "TV ↦data". iSplit; eauto.
-    steps_r. iDestruct "GRT" as "[[%V2 [[-> %Hle] [↦data TV]]] ->]".
+    steps_r. iDestruct "GRT" as "[-> [%V2 [[-> %Hle] [↦data TV]]]]".
     hss_r. steps_r.
 
     (* yield *)
-    iApply wsim_system_yield; ss.
-    { unfold_sp_exact sp_s SystemHdr.yield; ss. }
+    iApply wsim_system_yield_ir; ss. { simpl_sp; ss. }
     iFrame "TV IST".
     clear dependent st_src st_tgt.
     iIntros (??) "IST TV".
     steps_r.
-    Unshelve. all: try exact ⊤.
 
     (* open invariant *)
-    (* iMod (AtomicPtsToX_from_na _  _ V2 with "↦data") as "[%γd [%f [%t [%Hft [%V0 [% [%H02 [sw swX]]]]]]]]". *)
     iInv "I" as "INV" "ACC".
-    iEval (rewrite MPA.mp_inv'_eq /MPA.mp_inv'_def; SL_red) in "INV".
-    do 8 (iDestruct "INV" as "[% INV]"; iEval (SL_red) in "INV").
-    iDestruct "INV" as "[↦flag _]".
+    iEval (rewrite MPA.mp_inv'_eq /MPA.mp_inv'_def; solve_base_sl_red) in "INV".
+    iDestruct "INV" as "[% [%x0 [% [% [% [% [% [% [↦flag H]]]]]]]]]".
     rewrite syn_AtomicPtsTo_red.
     rewrite shift_0; iPoseProof (AtomicPtsTo_SWriter_agree with "[$] [$]") as "->".
 
     inline_r. steps_r.
     iEval (rewrite AtomicPtsTo_eq /AtomicPtsTo_def /view_at) in "↦flag".
     iDestruct "↦flag" as "[% ↦flag]".
-    force_r (existT 1 (tid, stid, loc, Val.Vnum 1, Ordering.acqrel, V2, γx, _, _, _, _, _, _, _)).
+    unshelve force_r.
+    { econs; right;
+        eexists (tid, stid, loc, Val.Vnum 1, Ordering.acqrel, V2, γx, _, _, _, _, _, _, _).
+      split; ss.
+    }
     forces_r.
     iFrame "↦flag". iSplitL "⊒ TV"; eauto.
     { iSplit; eauto. iSplit; eauto. iFrame. tview_sync Hle.
@@ -408,28 +367,24 @@ Module MPIA. Section MPIA.
     Unshelve. all: try exact 1%Qp.
     steps_r.
 
-    iDestruct "GRT" as "[[% [% [% [% [% [% [[-> [%Htime %Hres]] [sn [at [sy [swX tv]]]]]]]]]]] ->]".
+    iDestruct "GRT" as "[-> [% [% [% [% [% [% [[-> [%Htime %Hres]] [sn [at [sy [swX tv]]]]]]]]]]]]".
     destruct (Ordering.le _ _) eqn : Heqb in Hres; ss; subst; clear Heqb.
     rewrite Cell.max_ts_singleton in Htime.
-    hss_r. steps_r.
+    des; subst. hss_r. steps_r.
     iMod ("ACC" with "[↦data swX]") as "_".
     { rewrite MPA.mp_inv'_eq.
-      SL_red; iExists _; SL_red; iExists true.
-      do 6 (SL_red; iExists _).
-      SL_red.
-      rewrite syn_AtomicPtsTo_red; iFrame.
-      iSplitL "swX".
+      iEval solve_base_sl_red; iExists _, true; repeat iExists _.
+      rewrite syn_AtomicPtsTo_red; iSplitL "swX".
       { rewrite AtomicPtsTo_eq /AtomicPtsTo_def /view_at; iExists t; iFrame. }
-      do 3 (SL_red; iExists _); SL_red.
+      solve_base_sl_red; repeat iExists _.
       iSplitR "↦data".
-      iPureIntro. split; cycle 1; eauto.
+      { iPureIntro. split; eauto. }
       iRight; rewrite syn_own_loc_na_red.
       iApply (own_loc_mon_pred_gen with "↦data"); eauto; try exact 1%Qp.
       apply View.join_l.
     }
 
-    iApply wsim_system_yield; ss.
-    { unfold_sp_exact sp_s SystemHdr.yield; ss. }
+    iApply wsim_system_yield_ir; ss. { simpl_sp; ss. }
     iFrame "tv IST". clear dependent st_src st_tgt; iIntros (st_src st_tgt) "IST TID".
     steps_r.
 
@@ -438,25 +393,23 @@ Module MPIA. Section MPIA.
   Unshelve. all: try exact ⊤.
   Qed.
 
-  Lemma sim : ISim.t open MA MI MPA.init_cond IstFull.
+  Lemma sim : ISim.t open MA MI emp%I IstFull.
   Proof.
     init_sim.
     { eapply simF_mp2. }
     { eapply simF_mp. }
+    { iIntros "_"; repeat iExists _; repeat iSplit; eauto. }
   Qed.
 End MPIA.
 Section ctxr.
   Context `{!crisG Γ Σ α β τ _S _I, !concG, !histG, !atomicG, !sysG, !one_shotG}.
 
-  Definition ctxr (sp_s : sp_type) (sp_user : spl_type) :
-    sp_incl (SystemA.sp sp_user ⊤) sp_s →
-    spl_sub MPA.sp sp_user →
+  Definition ctxr (sp_s sp_user : specmap) :
+    (SystemA.sp sp_user ⊤) ⊆ sp_s →
+    MPA.sp ⊆ sp_user →
     ctx_refines
-      ((MPA.t sp_s ★ SystemA.t sp_user sp_s ★ PFMemA.t sp_s), MPA.init_cond)
-      ((MPI.t      ★ SystemA.t sp_user sp_s ★ PFMemA.t sp_s), True%I).
-  Proof using.
-    intros ??.
-    eapply main_adequacy, sim; eauto.
-  Qed.
+      ((MPA.t sp_s ★ SystemA.t sp_user ⊤ sp_s ★ PFMemA.t sp_s), emp%I)
+      ((MPI.t      ★ SystemA.t sp_user ⊤ sp_s ★ PFMemA.t sp_s), True%I).
+  Proof using. intros ??; eapply main_adequacy, sim; eauto. Qed.
 End ctxr.
 End MPIA.
