promise_free/system/SystemIARead.v
@@ -5,45 +5,33 @@ Require Import PFMemHeader PFMemA HistoryRA AtomicRA.
 Section SystemIA.
   Import SystemA.
   Context `{!crisG Γ Σ α β τ _S _I, !concG, !histG, !atomicG, !sysG}.
-  Context (sp_user : spl_type).
-  Context (sp : sp_type).
+  Context (sp_user sp : specmap).
   Context (size : list Z).
-  Context (Hincl : sp_incl sp_user sp).
-  Context (Hsysincl : sp_incl (SystemA.sp sp_user ⊤) sp).
+  Context (Hincl : sp_user ⊆ sp).
+  Context (Hsysincl : (SystemA.sp sp_user ⊤) ⊆ sp).
 
-  Local Definition SystemA_s := SystemA.t sp_user sp ★ PFMemA.t sp.
+  Local Definition SystemA_s := SystemA.t sp_user ⊤ sp ★ PFMemA.t sp.
   Local Definition SystemI_s := SystemI.t ★ PFMemA.t sp.
   Local Definition init_cond := init_cond size.
 
-  Definition Ist : alist key Any.t → alist key Any.t → iProp Σ :=
+  Definition Ist : ist_type Σ :=
     λ st_src st_tgt,
       (∃ (tid : Ident.t) (tids : gmap Ident.t (TView.t * nat)),
         let tids' : gmap Ident.t nat := snd <$> tids in
-        ⌜st_tgt = [(SystemI.v_tid, tid↑); (SystemI.v_tids, tids'↑)] ∧
-         st_src = [(SystemA.v_tid, tid↑); (SystemA.v_tids, tids'↑)]⌝ ∗
+        ⌜st_tgt = {[SystemI.v_tid := Some tid↑; SystemI.v_tids := Some tids'↑]} ∧
+         st_src = {[SystemI.v_tid := Some tid↑; SystemI.v_tids := Some tids'↑]}⌝ ∗
         tview_sys_auth tids ∗
         ([∗ map] i ↦ stid ∈ (snd <$> delete tid tids),
           (YIELD stid)))%I.
 
-  (* Definition Ist : alist key Any.t → alist key Any.t → iProp Σ :=
-    λ st_src st_tgt,
-      (∃ (tid : Ident.t) (tids : gmap Ident.t (TView.t * nat)) (flag : bool),
-        let tids' : gmap Ident.t nat := snd <$> tids in
-        ⌜st_tgt = [(SystemI.v_tid, tid↑); (SystemI.v_tids, tids'↑)] ∧
-         st_src = [(v_internal, flag↑); (SystemI.v_tid, tid↑); (SystemI.v_tids, tids'↑)]⌝ ∗
-        (if flag then winv (⊤, ⊤) else True) ∗
-        tview_sys_auth (fst <$> tids) ∗
-        [∗ map] tid ↦ 𝓥 ∈ fst <$> (if flag then tids else delete tid tids),
-          tview_sys_gen (1/2) tid 𝓥)%I. *)
+  Local Definition IstFull := (IstProd (IstSB (Mod.scopes (SystemA.t sp_user ⊤ sp)) Ist) IstEq).
 
-  Local Definition IstFull := (IstProd (IstSB (Mod.scopes (SystemA.t sp_user sp)) Ist) IstEq).
-
-  Lemma simF_read : ISim.sim_fun open SystemA_s SystemI_s init_cond IstFull (Some SystemHdr.read).
-  Proof.
-    init_simF.
-    steps_l. destruct _q as [[|[|i]] X]; steps_l; rename _q0 into arg'.
+  Lemma simF_read : ISim.sim_fun open SystemA_s SystemI_s IstFull (Some SystemHdr.read).
+  Proof using.
+    iStartSim.
+    steps_l. destruct _q as [? ? [[X [-> ->]]|[X [-> ->]]]]; steps_l; unfold_pre_post.
     { ss; destruct X as [[[[[[tid stid] loc] ord] val] q] V]; ss.
-      iDestruct "ASM" as "[[-> [PT TV]] ->]".
+      iDestruct "ASM" as "[-> [-> [PT TV]]]".
       iDestruct "TV" as "[TV STV]".
       iDestruct "IST" as (????) "[[-> ->] [[% IST] ->]]".
       iDestruct "IST" as "[%tid_cur [%tids [[-> ->] [TA YS]]]]".
@@ -54,18 +42,15 @@ Section SystemIA.
         iDestruct "STV" as "[_ Y2]"; iPoseProof (YieldToken_both with "Y2 TV2") as "%"; done.
       }
       subst.
-      (* destruct flag.
-      { iPoseProof (big_sepM_lookup_acc with "TVSM") as "[TVS2 TVSM]"; eauto.
-        iCombine "TVS TVS2" gives %[WF _]%gmap_view.gmap_view_frag_op_valid.
-        by apply dfrac_valid_own in WF.
-      } *)
+
       steps_r. hss_r. steps_r. rewrite /SystemI.get_tid. steps_r. hss_r. steps_r.
-      inline_r. force_r (existT 0 _). forces_r.
-      instantiate (1 := (tid_cur, loc, ord, val, q, V)); ss; iFrame.
-      iDestruct "TA" as "[TA TVS]".
+      inline_r. 
+      unshelve force_r (FSpec_mk _ _ (or_introl _)).
+      3:{ eexists (tid_cur, loc, ord, val, q, V); split; ss. }
+      forces_r. iFrame. iDestruct "TA" as "[TA TVS]".
       rewrite big_sepM_delete //=. iDestruct "TVS" as "[$ TVS]"; eauto.
       iSplit; eauto.
-      steps_r. iDestruct "GRT" as "[[%v [%V' [[-> %] [↦ tv]]]] ->]".
+      steps_r. iDestruct "GRT" as "[-> [%v [%V' [[-> %] [↦ tv]]]]]".
       iCombine "TA" "TV" as "TA".
       iMod (own_update with "TA") as "TA".
       { rewrite (gmap_view_replace _ tid_cur _ (to_agree _)) //. }
@@ -74,12 +59,12 @@ Section SystemIA.
       forces_l. iFrame. iSplit; eauto.
       step.
       iSplit; eauto.
-      iExists [_; _], [_; _], _, _; iSplit; eauto.
+      iExists _, _, _, _; iSplit; eauto.
       iSplit; eauto.
       iSplit; eauto.
-      (* rewrite lookup_fmap_Some in Hlookup; destruct Hlookup as [[? tid_s] [? Hlookup]]; ss; subst. *)
       iExists tid_cur, (<[tid_cur := (V', stid)]> tids); iSplit.
-      { iPureIntro; rewrite ?fmap_insert /= ?insert_id // lookup_fmap Hlookup //. }
+      { iPureIntro; split; rewrite ?fmap_insert /=; f_equal;
+          rewrite ?insert_id // lookup_fmap Hlookup //. }
       rewrite -fmap_insert /=; iFrame. rewrite delete_insert_delete.
       iSplitL "TVS tv"; eauto.
       rewrite big_sepM_insert_delete; iFrame.
@@ -87,7 +72,7 @@ Section SystemIA.
     { ss.
       destruct X as [[[[[[[[[[[tid stid] loc] ord] ζ] ζ'] t0] γ] tx] mode] V] Vb].
       ss; unfold_pre_post.
-      iDestruct "ASM" as "[[[-> %] [SN [PTS [Tid STid]]]] ->]".
+      iDestruct "ASM" as "[-> [[-> %] [SN [PTS [Tid STid]]]]]".
       iDestruct "IST" as (????) "[[-> ->] [[% IST] ->]]".
       iDestruct "IST" as "[%tid_cur [%tids [[-> ->] [TA YS]]]]". hss_r. steps_r.
       iPoseProof (tview_sys_lookup with "TA Tid") as "%Hlookup"; first iFrame.
@@ -97,28 +82,15 @@ Section SystemIA.
         iDestruct "STid" as "[_ Y2]"; iPoseProof (YieldToken_both with "Y2 TV2") as "%"; done.
       }
       subst.
-      (* iDestruct "IST" as "[%tid_cur [%tids [%flag [[-> ->] [W [[TA TVM] TVSM]]]]]]".
-      iPoseProof (tview_sys_lookup with "[TA TVM] TVS") as "%Hlookup"; first iFrame.
-      destruct (decide (tid = tid_cur)); cycle 1.
-      { iPoseProof (big_sepM_lookup_acc with "TVSM") as "[TV2 TVSM]".
-        { destruct flag; eauto. by rewrite fmap_delete lookup_delete_ne. }
-        iCombine "TVS TV2" gives %[WF _]%gmap_view.gmap_view_frag_op_valid.
-        by apply dfrac_valid_own in WF.
-      }
-      subst. *)
-      (* destruct flag.
-      { iPoseProof (big_sepM_lookup_acc with "TVSM") as "[TVS2 TVSM]"; eauto.
-        iCombine "TVS TVS2" gives %[WF _]%gmap_view.gmap_view_frag_op_valid.
-        by apply dfrac_valid_own in WF.
-      } *)
-      (* steps_r. hss_r. steps_r. *)
       rewrite /SystemI.get_tid. steps_r. hss_r. steps_r.
-      inline_r. force_r (existT 1 (tid_cur, loc, ord, _, _, _, _, _, _, _, _)).
+      inline_r.
+      unshelve force_r (FSpec_mk _ _ (or_intror _)).
+      3:{ eexists (tid_cur, loc, ord, _, _, _, _, _, _, _, _); split; ss. }
       forces_r. iFrame.
       iDestruct "TA" as "[TA TVS]".
       rewrite big_sepM_delete //. iDestruct "TVS" as "[$ TVS]"; eauto.
       iSplit; eauto.
-      steps_r. iDestruct "GRT" as "[[% [% [% [% [% [% [% [[-> %] [SN [PTS TV]]]]]]]]]] ->]".
+      steps_r. iDestruct "GRT" as "[-> [% [% [% [% [% [% [% [[-> %] [SN [PTS TV]]]]]]]]]]]".
       iCombine "TA" "Tid" as "TA".
       iMod (own_update with "TA") as "TA".
       { rewrite (gmap_view_replace _ tid_cur _ (to_agree _)) //. }
@@ -128,17 +100,16 @@ Section SystemIA.
       iPureIntro; des; esplits; eauto.
       step.
       iSplit; eauto.
-      iExists [_; _], [_; _], _, _; iSplit; eauto.
+      iExists _, _, _, _; iSplit; eauto.
       iSplit; eauto.
       iSplit; eauto.
-      (* rewrite lookup_fmap_Some in Hlookup; destruct Hlookup as [[? tid_s] [? Hlookup]]; ss; subst. *)
       iExists tid_cur, (<[tid_cur := (_, stid)]> tids); iSplit.
-      { iPureIntro; rewrite ?fmap_insert /= ?insert_id // lookup_fmap Hlookup //. }
+      { iPureIntro; split; rewrite ?fmap_insert /=; f_equal;
+          rewrite ?insert_id // lookup_fmap Hlookup //. }
       rewrite -fmap_insert /=; iFrame. rewrite delete_insert_delete.
       iSplitL "TVS TV"; eauto.
       rewrite big_sepM_insert_delete; iFrame.
     }
-    { destruct i; ss. }
   Unshelve. exact 1%Qp.
-  Qed.
+  (*SLOW*)Qed.
 End SystemIA.
