promise_free/system/SystemIAWrite.v
@@ -5,34 +5,33 @@ Require Import PFMemHeader PFMemA HistoryRA AtomicRA.
 Section SystemIA.
   Import SystemA.
   Context `{!crisG Γ Σ α β τ _S _I, !concG, !histG, !atomicG, !sysG}.
-  Context (sp_user : spl_type).
-  Context (sp : sp_type).
+  Context (sp_user sp : specmap).
   Context (size : list Z).
-  Context (Hincl : sp_incl sp_user sp).
-  Context (Hsysincl : sp_incl (SystemA.sp sp_user ⊤) sp).
+  Context (Hincl : sp_user ⊆ sp).
+  Context (Hsysincl : (SystemA.sp sp_user ⊤) ⊆ sp).
 
-  Local Definition SystemA_s := SystemA.t sp_user sp ★ PFMemA.t sp.
+  Local Definition SystemA_s := SystemA.t sp_user ⊤ sp ★ PFMemA.t sp.
   Local Definition SystemI_s := SystemI.t ★ PFMemA.t sp.
   Local Definition init_cond := init_cond size.
 
-  Definition Ist : alist key Any.t → alist key Any.t → iProp Σ :=
+  Definition Ist : ist_type Σ :=
     λ st_src st_tgt,
       (∃ (tid : Ident.t) (tids : gmap Ident.t (TView.t * nat)),
         let tids' : gmap Ident.t nat := snd <$> tids in
-        ⌜st_tgt = [(SystemI.v_tid, tid↑); (SystemI.v_tids, tids'↑)] ∧
-         st_src = [(SystemA.v_tid, tid↑); (SystemA.v_tids, tids'↑)]⌝ ∗
+        ⌜st_tgt = {[SystemI.v_tid := Some tid↑; SystemI.v_tids := Some tids'↑]} ∧
+         st_src = {[SystemI.v_tid := Some tid↑; SystemI.v_tids := Some tids'↑]}⌝ ∗
         tview_sys_auth tids ∗
         ([∗ map] i ↦ stid ∈ (snd <$> delete tid tids),
           (YIELD stid)))%I.
 
-  Local Definition IstFull := (IstProd (IstSB (Mod.scopes (SystemA.t sp_user sp)) Ist) IstEq).
+  Local Definition IstFull := (IstProd (IstSB (Mod.scopes SystemI.t) Ist) IstEq).
 
-  Lemma simF_write : ISim.sim_fun open SystemA_s SystemI_s init_cond IstFull (Some SystemHdr.write).
-  Proof.
-    init_simF.
-    steps_l. destruct _q as [[|[|i]] X]; steps_l; rename _q0 into arg'.
+  Lemma simF_write : ISim.sim_fun open SystemA_s SystemI_s IstFull (Some SystemHdr.write).
+  Proof using.
+    iStartSim.
+    steps_l. destruct _q as [? ? [[X [-> ->]]|[X [-> ->]]]]; steps_l; unfold_pre_post.
     { ss; destruct X as [[[[[tid stid] loc] val] ord] V]; ss.
-      iDestruct "ASM" as "[[-> [PT Tid]] ->]".
+      iDestruct "ASM" as "[-> [-> [PT Tid]]]".
       iDestruct "Tid" as "[Tid STV]".
       iDestruct "IST" as (????) "[[-> ->] [[% IST] ->]]".
       iDestruct "IST" as "[%tid_cur [%tids [[-> ->] [TA YS]]]]".
@@ -47,12 +46,14 @@ Section SystemIA.
       subst.
 
       steps_r. hss_r. steps_r. rewrite /SystemI.get_tid. steps_r. hss_r. steps_r.
-      inline_r. force_r (existT 0 _). forces_r.
-      instantiate (1 := (_, loc, val, ord, V)); ss; iFrame.
+      inline_r. rewrite /PFMemA.write_spec.
+      unshelve force_r (FSpec_mk _ _ (or_introl _)).
+      3:{ eexists (_, loc, val, ord, V); split; ss. }
+      forces_r. iFrame.
       iDestruct "TA" as "[TA TVS]".
-      rewrite big_sepM_delete //=. iDestruct "TVS" as "[$ TVS]"; eauto.
+      rewrite big_sepM_delete //=; iDestruct "TVS" as "[$ TVS]"; eauto.
       iSplit; eauto.
-      steps_r. iDestruct "GRT" as "[[%V' [[-> %] [↦ TV]]] ->]".
+      steps_r. iDestruct "GRT" as "[-> [%V' [[-> %] [↦ TV]]]]".
       iCombine "TA" "Tid" as "TA".
       iMod (own_update with "TA") as "TA".
       { rewrite (gmap_view_replace _ tid_cur _ (to_agree _)) //. }
@@ -63,18 +64,17 @@ Section SystemIA.
 
       (* IST *)
       iSplit; eauto.
-      iExists [_; _], [_; _], _, _; iSplit; eauto.
+      iExists _, _, _, _; iSplit; eauto.
       iSplit; eauto.
       iSplit; eauto.
       iExists tid_cur, (<[tid_cur := (V', stid)]> tids); iSplit.
-      { iPureIntro; rewrite ?fmap_insert /= ?insert_id // lookup_fmap Hlookup //. }
+      { iPureIntro; split; f_equal; rewrite fmap_insert /= insert_id // lookup_fmap Hlookup //. }
       rewrite -fmap_insert /=; iFrame. rewrite delete_insert_delete.
-      iSplitL "TVS TV"; eauto.
+      iFrame.
       rewrite big_sepM_insert_delete; iFrame.
     }
-    { ss.
-      destruct X as [[[[[[[[[[[[[tid stid] loc] val] ord] V] γ] ζ'] Vb] tx] ζ] mode] q] tx']; ss.
-      iDestruct "ASM" as "[[[-> %] [PT [PTS [Tid ?]]]] ->]".
+    { destruct X as [[[[[[[[[[[[[tid stid] loc] val] ord] V] γ] ζ'] Vb] tx] ζ] mode] q] tx']; ss.
+      iDestruct "ASM" as "[-> [[-> %] [PT [PTS [Tid ?]]]]]".
       iDestruct "Tid" as "[Tid STV]".
       iDestruct "IST" as (????) "[[-> ->] [[% IST] ->]]".
       iDestruct "IST" as "[%tid_cur [%tids [[-> ->] [TA YS]]]]".
@@ -89,12 +89,13 @@ Section SystemIA.
       subst.
 
       steps_r. hss_r. steps_r. rewrite /SystemI.get_tid. steps_r. hss_r. steps_r.
-      inline_r. force_r (existT 1 (tid_cur, loc, val, ord, V, γ, ζ', Vb, tx, ζ, mode, q, tx')).
+      inline_r. unshelve force_r (FSpec_mk _ _ (or_intror _)).
+      3:{ exists (tid_cur, loc, val, ord, V, γ, ζ', Vb, tx, ζ, mode, q, tx'). split; ss. }
       iDestruct "TA" as "[TA TVS]".
       forces_r. iFrame.
       rewrite big_sepM_delete //=. iDestruct "TVS" as "[$ TVS]"; eauto.
       iSplit; eauto.
-      steps_r. iDestruct "GRT" as "[[% [% [% [% [% [% [[-> %GRT] [? [? [? [? TV]]]]]]]]]]] ->]".
+      steps_r. iDestruct "GRT" as "[-> [% [% [% [% [% [% [[-> %GRT] [? [? [? [? TV]]]]]]]]]]]]".
       iCombine "TA" "Tid" as "TA".
       iMod (own_update with "TA") as "TA".
       { rewrite (gmap_view_replace _ tid_cur _ (to_agree _)) //. }
@@ -105,15 +106,16 @@ Section SystemIA.
 
       (* IST *)
       iSplit; eauto.
-      iExists [_; _], [_; _], _, _; iSplit; eauto.
+      iExists _, _, _, _; iSplit; eauto.
       iSplit; eauto.
       iSplit; eauto.
       iExists tid_cur, (<[tid_cur := (_, stid)]> tids); iSplit.
-      { iPureIntro; rewrite ?fmap_insert /= ?insert_id // lookup_fmap Hlookup //. }
+      { iPureIntro; split; rewrite fmap_insert /=; f_equal;
+          rewrite insert_id // lookup_fmap Hlookup //.
+      }
       rewrite -fmap_insert /=; iFrame. rewrite delete_insert_delete.
       iSplitL "TVS TV"; eauto.
       rewrite big_sepM_insert_delete; iFrame.
     }
-    { destruct i; ss. }
-  Qed.
+  (*SLOW*)Qed.
 End SystemIA.
