promise_free/pfmem/PFMemIA.v
@@ -15,11 +15,28 @@ Module PFMemIA. Section PFMemIA.
   Proof using.
     eapply main_adequacy with (Ist := PFMemIA.Ist).
     init_sim.
-    { split; first done. iIntros "[TVA [HA HFA]]"; ss.
+    { iIntros "[TVA [HA HFA]]"; ss.
       rewrite /PFMemIA.Ist.
       iExists (Global.init []), _, (View.init []); iSplit; cycle 1.
       { iFrame. rewrite Memory.cut_init //. }
-      { admit. }
+      iPureIntro; splits; ss.
+      { intros loc t f val V [-> [-> Hget]]%Memory.init_get Hacc.
+        rewrite /Memory.init /Memory.accessible /= /Block.accessible /= in Hacc.
+        repeat case_match; ss;
+          bsimpl; destruct Hacc as [?%Z.leb_le ?%Z.ltb_lt]; clarify; lia.
+      }
+      { apply Memory.closed_view_init. }
+      { apply Configuration.init_wf; auto. }
+      { intros loc Hpre.
+        rewrite /Memory.is_prealloced /Block.is_prealloced in Hpre.
+        rewrite /Memory.get_cell /=; des_ifs; ss.
+      }
+      { intros tid l lc; rewrite IdentMap.Facts.mapi_o; cycle 1.
+        { ii; subst; ss. }
+        destruct (decide (tid = 1%positive)); subst; ss.
+        { i; clarify; ss. }
+        rewrite IdentMap.singleton_neq //=.
+      }
     }
     { apply simF_alloc. }
     { apply simF_free. }
@@ -28,5 +45,5 @@ Module PFMemIA. Section PFMemIA.
     { apply simF_cas. }
     { apply simF_fence. }
     { apply simF_spawn. }
-  Admitted.
+  Qed.
 End PFMemIA. End PFMemIA.
