promise_free/pfmem/PFMemIARead.v
@@ -14,13 +14,14 @@ Section read.
   Definition MA := (PFMemA.t sp).
   Definition MI := (PFMemI.t syn size).
 
-  Lemma simF_read : ISim.sim_fun open MA MI (init_cond syn size) PFMemIA.Ist (Some PFMemHdr.read).
+  Lemma simF_read : ISim.sim_fun open MA MI PFMemIA.Ist (Some PFMemHdr.read).
   Proof.
-    init_simF.
-    step_l. destruct _q as [[|i] X]; steps_l; rename _q into arg'.
+    iStartSim.
+    step_l. destruct _q as [? ? [? | ?]].
     { (* non-atomic read *)
-      destruct X as [[[[[tid loc] ord] val] q] 𝓥].
-      iDestruct "ASM" as "[[-> [PT TV]] ->]". hss.
+      steps_l. rename _q into varg.
+      destruct f as [[[[[[tid loc] ord] val] q] 𝓥] [-> ->]]. unfold_pre_post.
+      iDestruct "ASM" as "[-> [-> [PT TV]]]". hss_r. steps_r.
       iDestruct "IST" as "[%gl [%ths [%Vcut [[-> [%CUT [%CUTCL [%WF [%WF2 [%PFG %PFL]]]]]] [HA [TA FA]]]]]]".
       steps_r. hss. steps_r.
       rewrite /PFMemI.check_ident.
@@ -29,7 +30,7 @@ Section read.
       destruct e; inv EVREAD; inv STEP; clear EVENT; rename STEP0 into STEP; s in STEP; cycle 1.
       { (* RACY READ *)
         inv STEP; inv LOCAL. inv LOCAL0. inv RACE.
-        { inv PFG; rewrite H2 in GET; ss. }
+        { inv PFG; rewrite H4 in GET; ss. }
         iPoseProof (tview_both_valid with "TA TV") as "%IN".
         destruct IN as [l [lc [FOUND LCEQ]]].
         s; rewrite FOUND in Heq; inv Heq.
@@ -43,7 +44,7 @@ Section read.
         assert (LECUT: Time.lt (View.rlx Vcut loc) to0).
         { inv SEEN_LOCAL.
           { ett. eapply l. etrans; eauto. }
-          { ett. eapply l. inv H2; eauto. }
+          { ett. eapply l. inv H4; eauto. }
         }
         assert (CUT_GET: Cell.get to0 (Cell.singleton (Message.message val V' na') LT) = Some (from, Message.message val0 released na)).
         { rewrite CELL_CUT Cell.cut_spec; des_ifs; timetac. }
@@ -61,12 +62,12 @@ Section read.
         exfalso; inv RACE; try done.
         hexploit (PFL tid); eauto; clear PFL; intros PFL.
         inv PFL; inv PFG.
-        des; rewrite H5 H6 in FREEPROMISE.
+        des; rewrite H7 H8 in FREEPROMISE.
         rewrite Promises.FreePromises.minus_bot in FREEPROMISE. inv FREEPROMISE.
       }
       (* VALID READ *)
       inv STEP; inv LOCAL. des_ifs. clear n.
-      steps_r. rewrite /alist_upd /_alist_upd /=.
+      steps_r.
       iPoseProof (tview_both_valid with "TA TV") as "%F"; des; subst.
       rewrite F in Heq; inv Heq.
 
@@ -84,7 +85,7 @@ Section read.
         assert (LECUT: Time.le (View.rlx Vcut loc) ts).
         { inv READABLE. inv SEEN_LOCAL.
           { etrans. eapply l. rewrite Time.le_lteq; left; tet; eauto. }
-          { etrans. eapply l. inv H2. eauto. }
+          { etrans. eapply l. inv H4. eauto. }
         }
 
         assert (CUT_GET: Cell.get ts (Cell.singleton (Message.message val V' na') LT) = Some (from, Message.message val'0 released na)).
@@ -98,9 +99,9 @@ Section read.
       inv LOCAL0.
       assert (EQ: val'0 = val ∧ V' = released ∧ na' = na ∧ from' = from).
       { rewrite Memory.get_memory_cell in CELL_GET'; des_ifs. }
-      destruct EQ as [H2 [H3 [H4 H5]]]; subst.
+      destruct EQ as [H4 [H5 [H6 H7]]]; subst.
       
-      remember ([(_, _)]) as st_tgt.
+      remember ({[_ := _]}) as st_tgt.
       iAssert (Ist st_src st_tgt)%I with "[HA FA TA]" as "IST".
       { iFrame. iPureIntro; esplits; eauto.
         { hexploit (@PFConfiguration.step_future ThreadEvent.get_machine_event); eauto.
@@ -113,9 +114,9 @@ Section read.
           i; des; eauto.
         }
         { i. destruct (decide (tid0 = tid)).
-          { subst. rewrite IdentMap.gss in H2; inv H2.
+          { subst. rewrite IdentMap.gss in H4; inv H4.
             hexploit PFL; eauto. }
-          { rewrite IdentMap.gso in H2; eauto. }
+          { rewrite IdentMap.gso in H4; eauto. }
         }
       }
 
@@ -123,13 +124,11 @@ Section read.
       iSplitR "IST".
       { iFrame. iSplit; eauto. iExists val'.
         iSplit; eauto.
-        rewrite own_loc_na_eq /own_loc_na_def /view_at.
-        iExists from, ts, LT, released, na.
         iSplit.
         { iSplit; eauto. 
-          iPureIntro; rewrite /alloc_local; split.
-          { ss. do 2 eapply AllocView.join_l; eauto. }
-          { eexists ts, (from, Message.message val released na).
+          (* iPureIntro; rewrite /alloc_local. *)
+          { ss. iPureIntro. do 2 eapply AllocView.join_l; eauto. }
+          { iPureIntro. eexists ts, (from, Message.message val released na).
             rewrite Cell.singleton_get; des_ifs.
             split; ss.
             unfold seen_local in *.
@@ -140,9 +139,9 @@ Section read.
       }
       step. iSplit; eauto.
     }
-    { destruct i; last (destruct i; inv X).
-      destruct X as [[[[[[[[[[tid loc] ord] ζ] ζ'] t] γ] q] mode] 𝓥] Vb].
-      iDestruct "ASM" as "[[[-> %ORDRLX] [SEEN [PT TV]]] ->]". hss.
+    { destruct f as [[[[[[[[[[[tid loc] ord] ζ] ζ'] t] γ] q] mode] 𝓥] Vb] [-> ->]].
+      steps_l. rename _q into varg.
+      iDestruct "ASM" as "[-> [[-> %ORDRLX] [SEEN [PT TV]]]]". hss_r.
       iDestruct "IST" as "[%gl [%ths [%Vcut [[-> [%CUT [%CUTCL [%WF [%WF2 [%PFG %PFL]]]]]] [HA [TA FA]]]]]]".
       steps_r. hss. steps_r.
       rewrite /PFMemI.check_ident.
@@ -227,7 +226,7 @@ Section read.
 
         iMod ((tview_auth_update ths (IdentMap.add tid (existT lang st2, lc2) ths)) with "TA TV") as "[TA TV]"; eauto.
 
-        remember ([(_, _)]) as st_tgt.
+        remember ({[_ := _]}) as st_tgt.
         iAssert (Ist st_src st_tgt)%I with "[HA FA TA]" as "IST".
         { iFrame. iPureIntro; esplits; eauto.
           { hexploit (@PFConfiguration.step_future ThreadEvent.get_machine_event); eauto.
@@ -237,10 +236,10 @@ Section read.
             i; des; eauto.
           }
           { i. destruct (decide (tid0 = tid)).
-            { subst. rewrite IdentMap.gss in H2; inv H2.
+            { subst. rewrite IdentMap.gss in H4; inv H4.
               hexploit PFL; eauto; intros PF. inv PF; des.
               econs; inv LOCAL0; eauto. }
-            { rewrite IdentMap.gso in H2; eauto. }
+            { rewrite IdentMap.gso in H4; eauto. }
           }
         }
 
@@ -286,14 +285,14 @@ Section read.
         iPoseProof (at_reader_extract with "R") as "#RR".
         { instantiate (1:=ζ'').
           ii. destruct (decide (to = ts)).
-          { subst. eapply Cell.add_get0 in H2. des.
+          { subst. eapply Cell.add_get0 in H4. des.
             rewrite GET1 in LHS. inv LHS.
             rewrite Cell.cut_spec.
             destruct (Time.le_lt_dec (View.rlx Vcut loc) ts); ss.
             timetac.
           }
-          { eapply Cell.add_o in H2. instantiate (1:=to) in H2.
-            rewrite LHS in H2. destruct (TimeSet.Facts.eq_dec to ts); ss.
+          { eapply Cell.add_o in H4. instantiate (1:=to) in H4.
+            rewrite LHS in H4. destruct (TimeSet.Facts.eq_dec to ts); ss.
             unfold Cell.le in LE. hexploit LE; eauto.
           }
         }
@@ -309,7 +308,7 @@ Section read.
             { subst. rewrite /seen_local.
               set (V := View.join _ _).
               enough (View.le (View.singleton loc ts) V).
-              { subst V. inv H4. ss.
+              { subst V. inv H6. ss.
                 eapply TimeMap.singleton_inv. ii.
                 specialize (RLX0 loc0). eauto.
               }
@@ -318,14 +317,14 @@ Section read.
                 eapply View.join_r.
               }
             }
-            { eapply Cell.add_o in H2. instantiate (1:=t0) in H2.
-              rewrite /is_Some in H3. des. destruct x. rewrite H3 in H2.
+            { eapply Cell.add_o in H4. instantiate (1:=t0) in H4.
+              rewrite /is_Some in H5. des. destruct x. rewrite H5 in H4.
               destruct (TimeSet.Facts.eq_dec t0 ts); ss.
               hexploit SEEN; eauto; i. unfold seen_local in *.
               etrans; eauto. etrans; eapply View.join_l.
             }
           }
-          { unfold good_absHist in *. ii. subst. inv H2.
+          { unfold good_absHist in *. ii. subst. inv H4.
             ss. assert (EX: None = Some (from, Message.message val' released na)).
             { rewrite -(Cell.bot_get ts) /Cell.bot /Cell.get /= CELL2.
               rewrite DOMap.gsspec.
@@ -337,7 +336,7 @@ Section read.
         }
 
         assert (GETTS0: Cell.get ts ζ'' = Some (from, msg)).
-        { inv H2; eauto. rewrite /Cell.get CELL2 DOMap.gsspec.
+        { inv H4; eauto. rewrite /Cell.get CELL2 DOMap.gsspec.
           destruct (DOMap.Properties.F.eq_dec ts ts); ss.
         }
 
@@ -375,7 +374,7 @@ Section read.
 
         iMod ((tview_auth_update ths (IdentMap.add tid (existT lang st2, lc2) ths)) with "TA TV") as "[TA TV]"; eauto.
 
-        remember ([(_, _)]) as st_tgt.
+        remember ({[_ := _]}) as st_tgt.
         iAssert (Ist st_src st_tgt)%I with "[HA FA TA]" as "IST".
         { iFrame. iPureIntro; esplits; eauto.
           { hexploit (@PFConfiguration.step_future ThreadEvent.get_machine_event); eauto.
@@ -389,9 +388,9 @@ Section read.
             i; des; eauto.
           }
           { i. destruct (decide (tid0 = tid)).
-            { subst. rewrite IdentMap.gss in H3; inv H3.
+            { subst. rewrite IdentMap.gss in H5; inv H5.
               hexploit PFL; eauto. }
-            { rewrite IdentMap.gso in H3; eauto. }
+            { rewrite IdentMap.gso in H5; eauto. }
           }
         }
 
@@ -410,9 +409,9 @@ Section read.
               rewrite /Memory.get /Block.get in GET.
               rewrite /Memory.get_cell. rewrite GET. eauto.
             }
-            { subst ts. eapply Cell.add_o with (t:= to) in H2.
+            { subst ts. eapply Cell.add_o with (t:= to) in H4.
               destruct (TimeSet.Facts.eq_dec to (Cell.max_ts ζ'')); ss.
-              rewrite H2 in GET0.
+              rewrite H4 in GET0.
               unfold Cell.le in LE. eapply LE in GET0.
               rewrite Cell.cut_spec in GET0.
               destruct (Time.le_lt_dec (View.rlx Vcut loc) to) eqn:L; ss.
@@ -429,5 +428,5 @@ Section read.
         step. iSplit; eauto.
       }
     }
-  Qed.
+  (*SLOW*)Qed.
 End read.
