promise_free/system/SystemTactics.v
@@ -3,35 +3,30 @@ Require Import CRIS SystemHeader SystemA.
 Section wsim.
   Context `{!crisG Γ Σ α β τ _S _I, !concG, !sysG}.
 
-  Lemma wsim_system_yield
+  Lemma wsim_system_yield_ir
       fl_src fl_tgt Ist r g R_src R_tgt RR p_src p_tgt
       st_src st_tgt itr_src itr_tgt
       (tid : Ident.t) (stid : nat) (V : TView.t)
-      (E E_src E_tgt : coPset)
-      (img_src img_tgt : bool)
-      (msk_src msk_tgt : string → bool)
-      scp_src sp_src
-      scp_tgt sp_tgt :
-    (E = if img_tgt then E_src ∖ E_tgt else E_src) →
-    E_tgt ⊆ E_src →
-    (img_tgt → img_src) →
-    msk_src SystemHdr.yield →
-    msk_tgt SystemHdr.yield →
-    (sp_src SystemHdr.yield = if img_src then Some (SystemA.yield_spec E_src) else None) →
-    (sp_tgt SystemHdr.yield = if img_tgt then Some (SystemA.yield_spec E_tgt) else None) →
+      (E : coPset)
+      (msk_src msk_tgt : emask)
+      sp_src sp_tgt :
+    sp_src !! speckey_fn SystemHdr.yield = fsp_some (SystemA.yield_spec E) →
+    sp_tgt !! speckey_fn SystemHdr.yield = None →
+    (∀ X, msk_tgt _ (subevent _ (Choose X))) →
+    (msk_tgt _ (subevent _ (Call SystemHdr.yield ()↑))) →
     Ist st_src st_tgt ∗
-    (if ((negb img_tgt) && img_src) then tview_sys tid stid V else emp) ∗
+    (tview_sys tid stid V) ∗
     (∀ st_src st_tgt,
       Ist st_src st_tgt -∗
-      (if ((negb img_tgt) && img_src) then tview_sys tid stid V else emp) -∗
+      (tview_sys tid stid V) -∗
       wsim fl_src fl_tgt Ist (E, E) r g R_src R_tgt RR true true
-        (st_src, SB.sandbox img_src msk_src scp_src (SModTr.trans true sp_src 𝒴) >>= itr_src)
+        (st_src, SB.sandbox msk_src (SModTr.trans sp_src 𝒴) >>= itr_src)
         (st_tgt, itr_tgt ())) ⊢
     wsim fl_src fl_tgt Ist (E, E) r g R_src R_tgt RR p_src p_tgt
-      (st_src, SB.sandbox img_src msk_src scp_src (SModTr.trans true sp_src 𝒴) >>= itr_src)
-      (st_tgt, SB.sandbox img_tgt msk_tgt scp_tgt (SModTr.trans false sp_tgt 𝒴) >>= itr_tgt).
+      (st_src, SB.sandbox msk_src (SModTr.trans sp_src 𝒴) >>= itr_src)
+      (st_tgt, SB.sandbox msk_tgt (SModTr.trans sp_tgt 𝒴) >>= itr_tgt).
   Proof.
-    intros -> ? Himg ?? Hsrc Htgt.
+    intros Hsps Hspt Hmsk Hcall.
     rewrite /System.yield; unseal "System".
     revert p_src. combine_quant p_tgt.
     combine_quant st_src. combine_quant st_tgt.
@@ -40,79 +35,50 @@ Section wsim.
     destruct_quant CIH.
 
     unfold_iterC_r.
-    steps_r. destruct _q as [[|]|]; cycle 2.
+    steps_r. rewrite Hmsk. steps_r. destruct _q as [[|]|]; cycle 2.
     { steps_r.
-      unfold_iterC_l. steps_l. force_l (Some false). steps_l.
-      iApply wsim_unfold; iIntros "W".
+      unfold_iterC_l.
+      steps_l. destruct (msk_src _); step_l; ss.
+      force_l (Some false). steps_l.
       iApply wsim_mono_knowledge; cycle 2.
-      { iApply wsim_fold; iFrame "W". iApply ("KTR" with "IST TV"). }
+      { iApply ("KTR" with "IST TV"). }
       { ii; iIntros "$ !> //". }
       { ii; iIntros "G"; iPoseProof (Hgg' with "G") as "$"; done. }
     }
-    { destruct img_tgt; cycle 1.
-      { steps_r. rewrite Htgt /=.
-        unfold_iterC_l. steps_l.
-        iApply wsim_progress.
-        force_l (Some true). steps_l.
-        destruct img_src; cycle 1.
-        { rewrite Hsrc /=. steps_l. steps_r.
-          call "IST".
-          steps_l. hss. steps_l.
-          steps_r. hss_r. step_r.
-          by_coind CIH.
-          iFrame.
-        }
-        { rewrite Hsrc /=.
-          force_l (tid, stid, V). steps_l. forces_l.
-          iFrame "TV". iSplit; eauto.
-          steps_l. steps_r.
-          call "IST".
-          steps_l. iDestruct "ASM" as "[[-> TV] ->]". hss.
-          steps_l. steps_r. hss_r. steps_r.
-          by_coind CIH.
-          iFrame.
-        }
-      }
-
-      destruct img_src; cycle 1.
-      { hexploit Himg; ss. }
-      steps_r. rewrite Htgt /=. steps_r.
-      iClear "TV"; iDestruct "GRT" as "[[-> TV] _]".
-
-      unfold_iterC_l. steps_l. force_l (Some true). steps_l.
-      rewrite Hsrc /=. force_l (_, _, _). steps_l.
-      rewrite difference_union_L (comm_L union) subseteq_union_1_L //.
-
-      forces_l. iFrame "TV". iSplit; eauto.
-      steps_l. call "IST".
-      steps_l. iDestruct "ASM" as "[[-> TV] ->]". hss.
-      steps_l. forces_r. iFrame "TV"; iSplit; eauto.
-      steps_r.
-      hss_r. steps_r.
-      by_coind CIH.
-      iFrame.
+    { steps_r. rewrite Hspt. steps_r. rewrite Hcall. steps_r.
+      unfold_iterC_l. steps_l. destruct (msk_src _); step_l; ss.
+      force_l (Some true). steps_l. rewrite Hsps /=.
+      step_l. destruct (msk_src _); step_l; ss. force_l (tid, stid, V).
+      step_l. destruct (msk_src _); step_l; ss. force_l.
+      step_l. destruct (msk_src _); step_l; ss. force_l.
+      iFrame "TV". iSplit; eauto.
+      step_l. destruct (msk_src _); step_l; ss.
+      call "IST".
+      clear st_src st_tgt. iIntros (ret st_src st_tgt) "IST".
+      step_l. destruct (msk_src _); step_l; ss.
+      step_l. destruct (msk_src _); steps_l; ss. steps_r.
+      by_coind CIH. iFrame. iDestruct "ASM" as "[? [? $]]".
     }
-    steps_r. unfold_iterC_l; steps_l; force_l (Some false); steps_l.
-    by_coind CIH.
-    iFrame.
+    unfold_iterC_l.
+    steps_l. destruct (msk_src _); step_l; ss. force_l (Some false). steps_l. steps_r.
+    by_coind CIH. iFrame.
   (*SLOW*)Qed.
 
   Lemma wsim_system_yield_src
       fl_src fl_tgt Ist r g R_src R_tgt RR p_src p_tgt
       st_src st_tgt itr_src itr_tgt
       (E : coPset)
-      (img_src : bool)
-      (msk_src : string → bool)
-      scp_src sp_src :
+      (msk_src : emask)
+      sp_src :
     wsim fl_src fl_tgt Ist (E, E) r g R_src R_tgt RR true p_tgt
       (st_src, itr_src ())
       (st_tgt, itr_tgt) ⊢
     wsim fl_src fl_tgt Ist (E, E) r g R_src R_tgt RR p_src p_tgt
-      (st_src, SB.sandbox img_src msk_src scp_src (SModTr.trans img_src sp_src 𝒴) >>= itr_src)
+      (st_src, SB.sandbox msk_src (SModTr.trans sp_src 𝒴) >>= itr_src)
       (st_tgt, itr_tgt).
   Proof.
     iIntros "S"; rewrite /System.yield; unseal "System".
     unfold_iterC_l; steps_l.
-    force_l (None); steps_l; done.
+    destruct msk_src; steps_l; ss. force_l (None); steps_l; done.
   Qed.
 End wsim.
